src/Quarantine.fst
@@ -1,0 +1,12 @@
+module Quarantine
+
+let quarantine_slab arr = if enable_quarantine_trap then trap_array arr else A.varray arr
+
+let mmap_trap_quarantine arr len =
+  if enable_quarantine_trap then (
+    mmap_trap arr len;
+    change_equal_slprop (trap_array arr) (quarantine_slab arr)
+  ) else (
+    noop ();
+    change_equal_slprop (A.varray arr) (quarantine_slab arr)
+  )
